get Impl to verify again

concurrency/node-replication/FlatCombinerTokens.i.dfy
@@ -1,5 +1,6 @@
 include "../framework/AsyncSSM.s.dfy"
 include "../../lib/Lang/NativeTypes.s.dfy"
+include "../../lib/Base/Option.s.dfy"
 include "Constants.i.dfy"
 
 module FlatCombinerTokens {
@@ -7,6 +8,7 @@ module FlatCombinerTokens {
   import opened NativeTypes
   import opened GhostLoc
   import opened Constants
+  import opened Options
 
   // Allows clients to enqueue requests
   // The combiner reads the requests and returns responses
@@ -18,11 +20,11 @@ module FlatCombinerTokens {
   
   datatype FCClient = FCClient(ghost loc: Loc, ghost tid: nat, ghost state: FCClientState)
 
-  datatype Elem = Elem(ghost tid: nat, ghost rid: nat)
+  datatype Elem = Elem(ghost rid: nat)
   datatype FCCombinerState =
     // no 'idle' state - just use Collecting(0, [])
-    | FCCombinerCollecting(ghost idx: nat, ghost elems: seq<Elem>)
-    | FCCombinerResponding(ghost idx: nat, ghost elems: seq<Elem>, ghost elem_idx: nat)
+    | FCCombinerCollecting(ghost elems: seq<Option<Elem>>)
+    | FCCombinerResponding(ghost elems: seq<Option<Elem>>, ghost idx: nat)
 
   datatype FCCombiner = FCCombiner(ghost loc: Loc, ghost state: FCCombinerState)
 
@@ -42,7 +44,7 @@ module FlatCombinerTokens {
     glinear slots: map<nat, FCSlot>,
     glinear combiner: FCCombiner
   )
-  ensures combiner.state == FCCombinerCollecting(0, [])
+  ensures combiner.state == FCCombinerCollecting([])
   ensures forall i | 0 <= i < MAX_THREADS_PER_REPLICA as int ::
       i in slots && slots[i] == FCSlot(combiner.loc, i, FCEmpty)
   ensures forall i | 0 <= i < MAX_THREADS_PER_REPLICA as int ::
@@ -51,63 +53,50 @@ module FlatCombinerTokens {
   glinear method combiner_collect(glinear comb: FCCombiner, glinear slot: FCSlot)
   returns (glinear comb': FCCombiner, glinear slot': FCSlot)
   requires comb.state.FCCombinerCollecting?
-  requires comb.state.idx < MAX_THREADS_PER_REPLICA as int
-  requires slot.tid == comb.state.idx
+  requires |comb.state.elems| < MAX_THREADS_PER_REPLICA as int
+  requires slot.tid == |comb.state.elems|
   requires comb.loc == slot.loc
   ensures slot.state.FCEmpty? || slot.state.FCRequest?
   ensures slot.state.FCEmpty? ==>
-      && comb' == FCCombiner(comb.loc, comb.state.(idx := comb.state.idx + 1))
+      && comb' == FCCombiner(comb.loc,
+          FCCombinerCollecting(comb.state.elems + [None]))
       && slot' == slot
   ensures slot.state.FCRequest? ==>
-      && comb' == FCCombiner(comb.loc, FCCombinerCollecting(comb.state.idx + 1,
-            comb.state.elems + [Elem(comb.state.idx, slot.state.rid)]))
+      && comb' == FCCombiner(comb.loc,
+          FCCombinerCollecting(
+            comb.state.elems + [Some(Elem(slot.state.rid))]))
       && slot' == slot.(state := FCInProgress(slot.state.rid))
     
   glinear method combiner_goto_responding(glinear comb: FCCombiner)
   returns (glinear comb': FCCombiner)
   requires comb.state.FCCombinerCollecting?
-  requires comb.state.idx == MAX_THREADS_PER_REPLICA as int
-  ensures comb' == FCCombiner(comb.loc, FCCombinerResponding(0, comb.state.elems, 0))
+  requires |comb.state.elems| == MAX_THREADS_PER_REPLICA as int
+  ensures comb' == FCCombiner(comb.loc, FCCombinerResponding(comb.state.elems, 0))
 
-  glinear method combiner_response_matches(glinear comb: FCCombiner, glinear slot: FCSlot)
-  returns (glinear comb': FCCombiner, glinear slot': FCSlot)
+  glinear method combiner_response_skip(glinear comb: FCCombiner)
+  returns (glinear comb': FCCombiner)
   requires comb.state.FCCombinerResponding?
-  requires comb.state.idx < MAX_THREADS_PER_REPLICA as int
-  requires slot.tid == comb.state.idx
-  requires slot.state.FCInProgress?
-  requires comb.loc == slot.loc
-  ensures 0 <= comb.state.elem_idx < |comb.state.elems|
-  ensures comb.state.elems[comb.state.elem_idx].tid == comb.state.idx
-  ensures comb' == comb && slot' == slot
-      
-  glinear method combiner_response_skip(glinear comb: FCCombiner, glinear slot: FCSlot)
-  returns (glinear comb': FCCombiner, glinear slot': FCSlot)
-  requires comb.state.FCCombinerResponding?
-  requires comb.state.idx < MAX_THREADS_PER_REPLICA as int
-  requires slot.tid == comb.state.idx
-  requires !slot.state.FCInProgress?
-  requires comb.loc == slot.loc
+  requires comb.state.idx < |comb.state.elems|
+  requires comb.state.elems[comb.state.idx].None?
   ensures comb' == FCCombiner(comb.loc, comb.state.(idx := comb.state.idx + 1))
-  ensures slot' == slot
 
   glinear method combiner_respond(glinear comb: FCCombiner, glinear slot: FCSlot)
   returns (glinear comb': FCCombiner, glinear slot': FCSlot)
   requires comb.state.FCCombinerResponding?
-  requires comb.state.idx < MAX_THREADS_PER_REPLICA as int
+  requires comb.state.idx < |comb.state.elems|
+  requires comb.state.elems[comb.state.idx].Some?
   requires slot.tid == comb.state.idx
-  requires 0 <= comb.state.elem_idx < |comb.state.elems|
-  requires comb.state.elems[comb.state.elem_idx].tid == comb.state.idx
   requires comb.loc == slot.loc
   ensures slot.state.FCInProgress?
-  ensures comb' == FCCombiner(comb.loc, comb.state.(idx := comb.state.idx + 1, elem_idx := comb.state.elem_idx + 1))
+  ensures comb' == FCCombiner(comb.loc, comb.state.(idx := comb.state.idx + 1))
   ensures slot' == slot.(state := FCResponse(slot.state.rid))
-  ensures comb.state.elems[comb.state.elem_idx].rid == slot.state.rid
+  ensures comb.state.elems[comb.state.idx].value.rid == slot.state.rid
 
   glinear method combiner_goto_collecting(glinear comb: FCCombiner)
   returns (glinear comb': FCCombiner)
   requires comb.state.FCCombinerResponding?
   requires comb.state.idx == MAX_THREADS_PER_REPLICA as int
-  ensures comb' == FCCombiner(comb.loc, FCCombinerCollecting(0, []))
+  ensures comb' == FCCombiner(comb.loc, FCCombinerCollecting([]))
 
   // Ops for the requester
 
@@ -132,4 +121,81 @@ module FlatCombinerTokens {
   ensures fc_client' == fc_client.(state := FCClientIdle)
   ensures fc_slot' == fc_slot.(state := FCEmpty)
 
+  //// Utilties for the impl
+
+  predicate RidsMatch(bools: seq<Option<Elem>>, rids: seq<RequestId>,
+      bools_start: nat,
+      bools_end: nat,
+      rids_start: nat,
+      rids_end: nat)
+  requires 0 <= bools_start <= bools_end <= |bools|
+  requires 0 <= rids_start <= rids_end <= |rids|
+  decreases bools_end
+  {
+    if bools_end == bools_start then (
+      rids_end == rids_start
+    ) else (
+      if bools[bools_end - 1].Some? then (
+        && rids_end > rids_start
+        && rids[rids_end - 1] == bools[bools_end - 1].value.rid
+        && RidsMatch(bools, rids, bools_start, bools_end - 1, rids_start, rids_end - 1)
+      ) else (
+        RidsMatch(bools, rids, bools_start, bools_end - 1, rids_start, rids_end)
+      )
+    )
+  }
+
+  lemma {:induction true} RidsMatchAddNone(bools: seq<Option<Elem>>, rids: seq<RequestId>,
+      bools_start: nat,
+      bools_end: nat,
+      rids_start: nat,
+      rids_end: nat)
+  requires 0 <= bools_start <= bools_end <= |bools|
+  requires 0 <= rids_start <= rids_end <= |rids|
+  requires RidsMatch(bools, rids, bools_start, bools_end, rids_start, rids_end)
+  ensures RidsMatch(bools+[None], rids, bools_start, bools_end, rids_start, rids_end)
+  {
+  }
+
+  lemma {:induction true} RidsMatchAddRidElem(bools: seq<Option<Elem>>, rids: seq<RequestId>,
+      bools_start: nat,
+      bools_end: nat,
+      rids_start: nat,
+      rids_end: nat,
+      rid: RequestId)
+  requires 0 <= bools_start <= bools_end <= |bools|
+  requires 0 <= rids_start <= rids_end <= |rids|
+  requires RidsMatch(bools, rids, bools_start, bools_end, rids_start, rids_end)
+  ensures RidsMatch(bools+[Some(Elem(rid))], rids+[rid], bools_start, bools_end, rids_start, rids_end)
+  {
+  }
+
+  lemma RidsMatchPop(bools: seq<Option<Elem>>, rids: seq<RequestId>,
+      bools_start: nat,
+      bools_end: nat,
+      rids_start: nat,
+      rids_end: nat)
+  requires 0 <= bools_start < bools_end <= |bools|
+  requires 0 <= rids_start <= rids_end <= |rids|
+  requires RidsMatch(bools, rids, bools_start, bools_end, rids_start, rids_end)
+  ensures bools[bools_start].Some? ==>
+      && rids_start < rids_end
+      && rids[rids_start] == bools[bools_start].value.rid
+      && RidsMatch(bools, rids, bools_start + 1, bools_end, rids_start + 1, rids_end)
+  ensures bools[bools_start].None? ==>
+      && RidsMatch(bools, rids, bools_start + 1, bools_end, rids_start, rids_end)
+  {
+    if bools_end == bools_start {
+    } else {
+      if bools[bools_end - 1].Some? {
+        if bools_end - 1 > bools_start {
+          RidsMatchPop(bools, rids, bools_start, bools_end - 1, rids_start, rids_end - 1);
+        }
+      } else {
+        if bools_end - 1 > bools_start {
+          RidsMatchPop(bools, rids, bools_start, bools_end - 1, rids_start, rids_end);
+        }
+      }
+    }
+  }
 }
